done (temporary)

Foundation/Modal/Logic/Extension.lean
@@ -28,6 +28,44 @@ lemma mem₂! (hφ : L₂ ⊢! φ) : sumQuasiNormal L₁ L₂ ⊢! φ := by
   apply iff_provable.mpr;
   apply sumQuasiNormal.mem₂ hφ;
 
+instance : Entailment.ModusPonens (sumQuasiNormal L₁ L₂) where
+  mdp hφψ hφ := by
+    constructor;
+    apply sumQuasiNormal.mdp;
+    . exact PLift.down hφψ;
+    . exact PLift.down hφ;
+
+instance : (sumQuasiNormal L₁ L₂).Substitution where
+  subst s hφ := by
+    constructor;
+    apply sumQuasiNormal.subst;
+    exact PLift.down hφ;
+
+lemma rec!
+  {motive : (φ : Formula α) → ((sumQuasiNormal L₁ L₂) ⊢! φ) → Sort}
+  (mem₁  : ∀ {φ}, (h : L₁ ⊢! φ) → motive φ (mem₁! h))
+  (mem₂  : ∀ {φ}, (h : L₂ ⊢! φ) → motive φ (mem₂! h))
+  (mdp   : ∀ {φ ψ : Formula α},
+           {hφψ : (sumQuasiNormal L₁ L₂) ⊢! φ ➝ ψ} → {hφ : (sumQuasiNormal L₁ L₂) ⊢! φ} →
+          motive (φ ➝ ψ) hφψ → motive φ hφ → motive ψ (hφψ ⨀ hφ)
+  )
+  (subst : ∀ {φ s}, {hφ : (sumQuasiNormal L₁ L₂) ⊢! φ} → (motive φ hφ) → motive (φ⟦s⟧) (Logic.subst! _ hφ))
+  : ∀ {φ}, (h : sumQuasiNormal L₁ L₂ ⊢! φ) → motive φ h := by
+  intro _ hφ;
+  induction (iff_provable.mp $ hφ) with
+  | mem₁ h => apply mem₁ h;
+  | mem₂ h => apply mem₂ h;
+  | mdp hφψ hφ ihφψ ihφ =>
+    apply mdp;
+    . apply ihφψ;
+    . apply ihφ;
+    . apply iff_provable.mpr; assumption;
+    . apply iff_provable.mpr; assumption;
+  | subst hφ ihφ =>
+    apply subst;
+    . apply ihφ;
+    . apply iff_provable.mpr; assumption;
+
 lemma symm : sumQuasiNormal L₁ L₂ = sumQuasiNormal L₂ L₁ := by
   ext φ;
   constructor;
@@ -46,15 +84,10 @@ lemma symm : sumQuasiNormal L₁ L₂ = sumQuasiNormal L₂ L₁ := by
 
 variable [DecidableEq α]
 
-instance [L₁.IsQuasiNormal] : Entailment.Lukasiewicz (sumQuasiNormal L₁ L₂) where
+instance [Entailment.Cl L₁] : Entailment.Lukasiewicz (sumQuasiNormal L₁ L₂) where
   imply₁ _ _ := by constructor; apply sumQuasiNormal.mem₁; simp;
   imply₂ _ _ _ := by constructor; apply sumQuasiNormal.mem₁; simp;
   elimContra _ _ := by constructor; apply sumQuasiNormal.mem₁; simp;
-  mdp hφψ hφ := by
-    constructor;
-    apply sumQuasiNormal.mdp;
-    . exact PLift.down hφψ;
-    . exact PLift.down hφ;
 
 instance [L₁.IsQuasiNormal] : (sumQuasiNormal L₁ L₂).IsQuasiNormal where
   K _ _ := by constructor; apply sumQuasiNormal.mem₁; simp;
@@ -70,8 +103,7 @@ instance [L₂.IsQuasiNormal] : (sumQuasiNormal L₁ L₂).IsQuasiNormal := by
 instance : L₁ ⪯ sumQuasiNormal L₁ L₂ := by
   apply weakerThan_iff.mpr;
   intro φ hφ;
-  apply iff_provable.mpr;
-  apply sumQuasiNormal.mem₁ hφ;
+  exact mem₁! hφ;
 
 instance : L₂ ⪯ sumQuasiNormal L₁ L₂ := by
   rw [sumQuasiNormal.symm];
@@ -81,103 +113,130 @@ end sumQuasiNormal
 
 
 inductive sumNormal (L₁ L₂ : Logic α) : Logic α
-  | mem₁ {φ}    : φ ∈ L₁ → sumNormal L₁ L₂ φ
-  | mem₂ {φ}    : φ ∈ L₂ → sumNormal L₁ L₂ φ
+  | mem₁ {φ}    : L₁ ⊢! φ → sumNormal L₁ L₂ φ
+  | mem₂ {φ}    : L₂ ⊢! φ → sumNormal L₁ L₂ φ
   | mdp  {φ ψ}  : sumNormal L₁ L₂ (φ ➝ ψ) → sumNormal L₁ L₂ φ → sumNormal L₁ L₂ ψ
   | subst {φ s} : sumNormal L₁ L₂ φ → sumNormal L₁ L₂ (φ⟦s⟧)
   | nec {φ}     : sumNormal L₁ L₂ φ → sumNormal L₁ L₂ (□φ)
 
-abbrev addNormal (L : Logic α) (φ : Formula α) : Logic α := sumNormal L {φ}
-
 namespace sumNormal
+
+variable {φ ψ : Formula α}
+
+lemma mem₁! (hφ : L₁ ⊢! φ) : sumNormal L₁ L₂ ⊢! φ := by
+  apply iff_provable.mpr;
+  apply sumNormal.mem₁ hφ;
+
+lemma mem₂! (hφ : L₂ ⊢! φ) : sumNormal L₁ L₂ ⊢! φ := by
+  apply iff_provable.mpr;
+  apply sumNormal.mem₂ hφ;
+
+instance : Entailment.ModusPonens (sumNormal L₁ L₂) where
+  mdp hφψ hφ := by
+    constructor;
+    apply sumNormal.mdp;
+    . exact PLift.down hφψ;
+    . exact PLift.down hφ;
+
+instance : Entailment.Necessitation (sumNormal L₁ L₂) where
+  nec hφ := by
+    constructor;
+    apply sumNormal.nec;
+    exact PLift.down hφ;
+
+instance : (sumNormal L₁ L₂).Substitution where
+  subst s hφ := by
+    constructor;
+    apply sumNormal.subst;
+    exact PLift.down hφ;
+
+
+lemma rec!
+  {motive : (φ : Formula α) → ((sumNormal L₁ L₂) ⊢! φ) → Sort}
+  (mem₁  : ∀ {φ}, (h : L₁ ⊢! φ) → motive φ (mem₁! h))
+  (mem₂  : ∀ {φ}, (h : L₂ ⊢! φ) → motive φ (mem₂! h))
+  (mdp   : ∀ {φ ψ : Formula α},
+           {hφψ : (sumNormal L₁ L₂) ⊢! φ ➝ ψ} → {hφ : (sumNormal L₁ L₂) ⊢! φ} →
+          motive (φ ➝ ψ) hφψ → motive φ hφ → motive ψ (hφψ ⨀ hφ)
+  )
+  (nec   : ∀ {φ}, {hφ : (sumNormal L₁ L₂) ⊢! φ} → (motive φ hφ) → motive (□φ) (Entailment.nec! hφ))
+  (subst : ∀ {φ s}, {hφ : (sumNormal L₁ L₂) ⊢! φ} → (motive φ hφ) → motive (φ⟦s⟧) (Logic.subst! _ hφ))
+  : ∀ {φ}, (h : sumNormal L₁ L₂ ⊢! φ) → motive φ h := by
+  intro _ hφ;
+  induction (iff_provable.mp $ hφ) with
+  | mem₁ h => apply mem₁ h;
+  | mem₂ h => apply mem₂ h;
+  | mdp hφψ hφ ihφψ ihφ =>
+    apply mdp;
+    . apply ihφψ;
+    . apply ihφ;
+    . apply iff_provable.mpr; assumption;
+    . apply iff_provable.mpr; assumption;
+  | nec hφ ihφ =>
+    apply nec;
+    . apply ihφ;
+    . apply iff_provable.mpr; assumption;
+  | subst hφ ihφ =>
+    apply subst;
+    . apply ihφ;
+    . apply iff_provable.mpr; assumption;
+
+lemma symm : sumNormal L₁ L₂ = sumNormal L₂ L₁ := by
+  ext φ;
+  constructor;
+  . intro h;
+    induction h with
+    | mem₁ h => exact sumNormal.mem₂ h;
+    | mem₂ h => exact sumNormal.mem₁ h;
+    | mdp _ _ ihφψ ihφ => exact sumNormal.mdp ihφψ ihφ;
+    | subst _ ihφ => exact sumNormal.subst ihφ;
+    | nec _ ihφ => exact sumNormal.nec ihφ;
+  . intro h;
+    induction h with
+    | mem₁ h => exact sumNormal.mem₂ h;
+    | mem₂ h => exact sumNormal.mem₁ h;
+    | mdp _ _ ihφψ ihφ => exact sumNormal.mdp ihφψ ihφ;
+    | subst _ ihφ => exact sumNormal.subst ihφ;
+    | nec _ ihφ => exact sumNormal.nec ihφ;
+
+variable [DecidableEq α]
+
+instance [Entailment.Cl L₁] : Entailment.Lukasiewicz (sumNormal L₁ L₂) where
+  imply₁ _ _ := by constructor; apply sumNormal.mem₁; simp;
+  imply₂ _ _ _ := by constructor; apply sumNormal.mem₁; simp;
+  elimContra _ _ := by constructor; apply sumNormal.mem₁; simp;
+  mdp hφψ hφ := by
+    constructor;
+    apply sumNormal.mdp;
+    . exact PLift.down hφψ;
+    . exact PLift.down hφ;
+
+instance [L₁.IsNormal] : (sumNormal L₁ L₂).IsNormal where
+  K _ _ := by constructor; apply sumNormal.mem₁; simp;
+  subst s hφ := by
+    constructor;
+    apply sumNormal.subst;
+    exact PLift.down hφ;
+  nec hφ := by
+    constructor;
+    apply sumNormal.nec;
+    exact PLift.down hφ;
+
+instance [L₂.IsNormal] : (sumNormal L₁ L₂).IsNormal := by
+  rw [sumNormal.symm];
+  infer_instance;
+
+instance : L₁ ⪯ sumNormal L₁ L₂ := by
+  apply weakerThan_iff.mpr;
+  intro φ hφ;
+  exact mem₁! hφ;
+
+instance : L₂ ⪯ sumNormal L₁ L₂ := by
+  rw [sumNormal.symm];
+  infer_instance;
 
 end sumNormal
 
 end Logic
-
-
-
-
-/-
-def QuasiNormalExtension (L : Logic) := { L' : Logic // L ⊆ L' ∧ L'.IsQuasiNormal }
-
-namespace QuasiNormalExtension
-
-variable {L₀ : Logic} {L : QuasiNormalExtension L₀}
-
-instance : Membership (Formula ℕ) (QuasiNormalExtension L₀) := ⟨λ L φ => φ ∈ L.1⟩
-
-lemma mem_of_mem_base (h : φ ∈ L₀) : φ ∈ L := L.property.1 h
-
-lemma mem_of_mem_LogicK (h : φ ∈ Logic.K) : φ ∈ L := L.property.2.subset_K h
-
-lemma mdp (hφψ : φ ➝ ψ ∈ L) (hφ : φ ∈ L) : ψ ∈ L := L.property.2.mdp_closed hφψ hφ
-
-lemma subst (hφ : φ ∈ L) : φ⟦s⟧ ∈ L := L.property.2.subst_closed hφ s
-
-def add (L₁ L₂ : QuasiNormalExtension L₀) : QuasiNormalExtension L₀ where
-  val := Logic.sumQuasiNormal L₁.1 L₂.1
-  property := by
-    constructor;
-    . intro φ hφ;
-      apply Logic.sumQuasiNormal.mem₁;
-      apply mem_of_mem_base hφ;
-    . refine ⟨?_, ?_, ?_⟩;
-      . intro φ hφ;
-        apply Logic.sumQuasiNormal.mem₁;
-        apply mem_of_mem_LogicK hφ;
-      . intro φ ψ hφ hφψ;
-        apply Logic.sumQuasiNormal.mdp hφ hφψ;
-      . intro φ hφ s;
-        apply Logic.sumQuasiNormal.subst hφ;
-
-instance : Add (QuasiNormalExtension L₀) := ⟨add⟩
-
-/-
-instance : Std.IdempotentOp (α := QuasiNormalExtension L₀) (· + ·) where
-  idempotent := by
-    intro L;
-    sorry;
-
-instance : Std.Commutative (α := QuasiNormalExtension L₀) (· + ·) where
-  comm := by
-    intro L₁ L₂;
-    sorry;
-
-instance : Std.Associative (α := QuasiNormalExtension L₀) (· + ·) where
-  assoc := by
-    intro L₁ L₂ L₃;
-    sorry;
--/
-
-def inter (L₁ L₂ : QuasiNormalExtension L₀) : QuasiNormalExtension L₀ where
-  val := L₁.1 ∩ L₂.1
-  property := by
-    constructor;
-    . intro φ hφ;
-      apply Set.mem_inter <;> exact mem_of_mem_base hφ;
-    . refine ⟨?_, ?_, ?_⟩;
-      . intro φ hφ;
-        apply Set.mem_inter <;> exact mem_of_mem_LogicK hφ;
-      . rintro φ ψ ⟨hφψ₁, hφψ₂⟩ ⟨hφ₁, hφ₂⟩;
-        apply Set.mem_inter;
-        . exact mdp hφψ₁ hφ₁;
-        . exact mdp hφψ₂ hφ₂;
-      . rintro φ ⟨hφ₁, hφ₂⟩ s;
-        apply Set.mem_inter;
-        . exact subst hφ₁;
-        . exact subst hφ₂;
-
-instance : Inter (QuasiNormalExtension L₀) := ⟨inter⟩
-
-end QuasiNormalExtension
-
-
-def ExtensionNormal (L : Logic) := { L' : Logic // L'.IsNormal ∧ L ⊆ L' }
-
-namespace ExtensionNormal
-
-end ExtensionNormal
--/
 
 end LO.Modal
